---
layout: post
title: "Proximal Operator"
excerpt: ""
categories: articles
tags: [convex optimization]
comments: true
share: true
---

Consider the following question

Show that if $$\forall y \in \operatorname{dom}(g)$, $\partial g(prox_f (y)) \supseteq \partial g(y)$$, then $$ prox_{f+g}(x) = prox_{f}(prox_{g}(x))$$


Proof:  

$$prox_{f+g} = argmin \frac{1}{2} ||z - x||_2^2 + f(z) + g(z)$$  

$$prox_{f} = argmin \frac{1}{2} ||z - x||_2^2 + f(z)$$

$$prox_{g} = argmin \frac{1}{2} ||z - x||_2^2 + g(z)$$

WTS $$prox_{f}(prox_{g}(x)) = argmin \frac{1}{2} ||prox_g(x) - z||_2^2 + f(z) = argmin \frac{1}{2} ||z - x||_2^2 + f(z) + g(z)$$ 

WTS $$0 \in z - prox_g(x) - \partial f(z)$$ and $$0 \in z - x + \partial f(z) + \partial g(z)$$


So the proof becomes if $$0 \in z - prox_g(x) - \partial f(z)$$, we need to prove $$0 \in z - x + \partial f(z) + \partial g(z)$$, and 
if $$0 \in z - x + \partial f(z) + \partial g(z)$$, then $$0 \in z - prox_g(x) - \partial f(z)$$


